examples/riscv/symbexectests/nestfunc_symb_execScript.sml
@@ -10,6 +10,13 @@ open nestfunc_specTheory;
 val _ = new_theory "nestfunc_symb_exec";
 
 (* --------------------------- *)
+(* prepare program lookups     *)
+(* --------------------------- *)
+
+val bir_lift_thm = birs_stepLib.patch_lifter_thm bir_nestfunc_riscv_lift_THM;
+val _ = birs_stepLib.prepare_program_lookups bir_lift_thm;
+
+(* --------------------------- *)
 (* Symbolic analysis execution *)
 (* --------------------------- *)
 
